---
title: "[Draft] It√¥'s lemma"
date: 2025-12-30 00:08:00+09:00
tags: [financial mathematics] # TAG names should always be lowercase
math: true
---

# Description

If $f \in C^2(\mathbb{R})$, then

$$
f(B(b)) - f(B(a)) = \int_a^b f'(B(t))\, dB(t) + \frac{1}{2}\int_a^b f''(B(t))\, dt.
$$

# Derivation

## Taylor expansion

Let $$\Pi_n = \{t_0,\, t_1,\, \cdots,\, t_n\}$$ be a partition of $[a, b]$, where $$a = t_0 < t_1 < \cdots < t_n = b$$.

$$
\begin{align*}
f(B(b)) - f(B(a)) &= \sum_{i=1}^n f(B(t_i)) - f(B(t_{i-1})) \\
&= \sum_{i=1}^n f'(B(t_{i-1}))(B(t_i) - B(t_{i-1})) + \frac{1}{2}\sum_{i=1}^n f''(\xi_{n,i})(B(t_i) - B(t_{i-1}))^2 \\
&= \sum_{i=1}^n f'(B(t_{i-1}))(B(t_i) - B(t_{i-1})) + \frac{1}{2} \underbrace{\sum_{i=1}^n (f''(\xi_{n,i}) - f''(B(t_{i-1})))(B(t_i) - B(t_{i-1}))^2}_{(1)} \\
&\quad + \frac{1}{2} \underbrace{\sum_{i=1}^n f''(B(t_{i-1}))((B(t_i) - B(t_{i-1}))^2 - (t_i - t_{i-1}))}_{(2)} \\
&\quad + \frac{1}{2}\sum_{i=1}^n f''(B(t_{i-1}))(t_i - t_{i-1}),
\end{align*}
$$

where $$\xi_{n,i} = B(t_{i-1}) + \lambda_i (B(t_i) - B(t_{i-1}))$$ for some $$\lambda_i \in (0, 1)$$.

## Error term (1)

Define

$$
\xi_n = \max_{1 \leq i \leq n,\, 0 < \lambda < 1} \left\vert f''(B(t_{i-1}) + \lambda (B(t_i) - B(t_{i-1}))) - f''(B(t_{i-1})) \right\vert .
$$

- Since $f''$ is uniformly continuous on any compact set, $\xi_n \to 0$ as $n \to \infty$ a.s.
- $\sum_{i=1}^n (B(t_i) - B(t_{i-1}))^2 \to b - a$ almost surely as $n \to \infty$.

## Error term (2)
